veric/rmaps_lemmas.v
@@ -45,16 +45,8 @@ Proof.
   inv H; auto.
 Qed.
 
-Lemma GHOST_identity: forall m, identity m -> identity (GHOST m).
-Proof.
-  repeat intro.
-  inv H0.
-  apply H in RJ; subst; auto.
-Qed.
-
 Lemma identity_NO:
-  forall r, identity  r -> r = NO Share.bot bot_unreadable \/ (exists k, exists pds, r = PURE k pds) \/
-    exists m, r = GHOST m /\ identity m.
+  forall r, identity  r -> r = NO Share.bot bot_unreadable \/ exists k, exists pds, r = PURE k pds.
 Proof.
   destruct r; auto; intros.
  * left.
@@ -64,13 +56,7 @@ Proof.
  * apply identity_unit' in H. inv H.
    apply unit_identity in RJ. apply identity_share_bot in RJ. subst.
    contradiction bot_unreadable.
- * right; left. exists k. exists p. trivial.
- * right; right.
-   do 2 eexists; eauto.
-   repeat intro.
-   spec H (GHOST a) (GHOST b); spec H.
-   constructor; auto.
-   inv H; auto.
+ * right. exists k. exists p. trivial.
 Qed.
 
 Lemma age1_resource_at_identity:
@@ -87,10 +73,9 @@ Proof.
   rewrite unsquash_squash.
   simpl.
   destruct r. simpl in *.
-  unfold compose; simpl. destruct H1 as [H1 | [[k [pds H1]] | [m [H1 Hm]]]]; rewrite H1; simpl; auto.
+  unfold compose; simpl. destruct H1 as [H1 | [k [pds H1]]]; rewrite H1; simpl; auto.
   apply NO_identity.
   apply PURE_identity.
-  apply GHOST_identity; auto.
  (* BACKWARD DIRECTION *)
   generalize (identity_NO _ H0); clear H0; intro.
   unfold resource_at in *. simpl in H.
@@ -101,11 +86,9 @@ Proof.
   unfold compose in H1; simpl in H1.
   unfold resource_fmap in H1.
   destruct (x loc).
-  destruct H1. inv H0;   apply NO_identity. destruct H0 as [[? [? H0]] | [? [H0 ?]]]; inv H0.
-  destruct H1 as [H1 | [[k' [pds' H1]] | [? [H1 ?]]]]; inv H1.
+  destruct H1. inv H0;   apply NO_identity. destruct H0 as [? [? H0]]; inv H0.
+  destruct H1 as [H1 | [k' [pds' H1]]]; inv H1.
   apply PURE_identity.
-  destruct H1 as [H1 | [[? [? H1]] | [? [H1 ?]]]]; inv H1.
-  apply GHOST_identity; auto.
 Qed.
 
 Lemma necR_resource_at_identity:
@@ -293,8 +276,6 @@ Proof.
    apply join_readable_part; auto. simpl. constructor; auto.
    *
    inv H3; constructor; auto.
-   *
-   inv H3; constructor.
   }
  destruct H4 as [phig [? ?]].
  exists phif; exists phig.
@@ -645,18 +626,6 @@ Proof.
   apply (necR_resource_at _ _ _ _ H H1).
 Qed.
 
-Lemma necR_GHOST:
-  forall phi phi' loc m,
-        necR phi phi' ->
-         phi @ loc = GHOST m ->
-         phi' @ loc = GHOST m.
-Proof.
-  intros.
-  generalize (eq_sym (resource_at_approx phi loc));
-  pattern (phi @ loc) at 2; rewrite H0; intro.
-  apply (necR_resource_at _ _ _ _ H H1).
-Qed.
-
 Lemma necR_NO:
    forall phi phi' l sh nsh, necR phi phi' -> 
    (phi@l = NO sh nsh <-> phi'@l = NO sh nsh).
@@ -668,13 +637,11 @@ Proof.
   generalize (necR_NOx _ _ l _ _ H H1); intro. congruence.
   generalize (necR_YES _ _ _ _ _ _ _ H H1); congruence.
   generalize (necR_PURE _ _ _ _ _ H H1); congruence.
-  generalize (necR_GHOST _ _ _ _ H H1); congruence.
 Qed.
 
 Lemma resource_at_empty: forall phi, 
      identity phi ->
-     forall l, (phi @ l = NO Share.bot bot_unreadable \/ (exists k, exists pds, phi @ l = PURE k pds) \/
-       exists m, phi @ l = GHOST m /\ identity m).
+     forall l, phi @ l = NO Share.bot bot_unreadable \/ exists k, exists pds, phi @ l = PURE k pds.
 Proof.
   intros.
   rewrite identity_unit_equiv in H.
@@ -688,9 +655,6 @@ Proof.
   clear - r RJ.
   apply share_self_join_bot in RJ. subst.
   contradiction (bot_unreadable r).
-  right; right.
-  do 2 eexists; eauto.
-  apply identity_unit_equiv; auto.
 Qed.
 Arguments resource_at_empty [phi] _ _.
 
@@ -798,20 +762,6 @@ split; intros [pp ?].
   eauto.
 Qed.
 
-Lemma necR_GHOST':
-   forall phi phi' l m, necR phi phi' -> 
-   (phi@l = GHOST m <-> phi'@l = GHOST m).
-Proof.
-  intros; split.
-  apply necR_GHOST; auto.
-  intros.
-  case_eq (phi @ l); intros.
-  generalize (necR_NOx _ _ l _ _ H H1); congruence.
-  generalize (necR_YES _ _ _ _ _ _ _ H H1); congruence.
-  generalize (necR_PURE _ _ _ _ _ H H1); congruence.
-  generalize (necR_GHOST _ _ _ _ H H1); congruence.
-Qed.
-
 
 Lemma resource_at_join_sub:
   forall phi1 phi2 l,
@@ -845,7 +795,6 @@ Proof.
   destruct p.
   rewrite (necR_YES phi phi' loc _ _ _ _ H H0); auto.
   rewrite (necR_PURE phi phi' loc _ _ H H0); auto.
-  rewrite (necR_GHOST phi phi' loc _ H H0); auto.
 Qed.
 
 
@@ -901,16 +850,7 @@ Proof.
   constructor 1; auto.
 Qed.
 
-Lemma age1_GHOST: forall phi phi' l m,
-  age1 phi = Some phi' -> ((phi @ l = GHOST m) <-> phi' @ l = GHOST m).
-Proof.
-  intros.
-  apply necR_GHOST'.
-  constructor 1; auto.
-Qed.
-
-Lemma empty_NO: forall r, identity r -> r = NO Share.bot bot_unreadable \/ (exists k, exists pds, r = PURE k pds)
-  \/ exists m, r = GHOST m /\ identity m.
+Lemma empty_NO: forall r, identity r -> r = NO Share.bot bot_unreadable \/ exists k, exists pds, r = PURE k pds.
 Proof.
 intros.
 destruct r; auto.
@@ -923,13 +863,7 @@ spec H.
 apply res_join_NO2.
 auto.
 inv H.
-right; left. exists k. exists p. trivial.
-right; right.
-do 2 eexists; eauto.
-repeat intro.
-spec H (GHOST a) (GHOST b); spec H.
-constructor; auto.
-inv H; auto.
+right. exists k. exists p. trivial.
 Qed.
 
 Lemma level_age_fash:
@@ -992,7 +926,6 @@ assert (AV.valid (res_option oo (fun loc => proj1_sig (H0 loc)))). {
  rewrite (join_readable_part_eq r nsh2 rsh3 RJ); constructor.
  constructor. apply join_readable_part; auto. split; reflexivity.
  inv j; constructor.
- inv j; constructor.
 }
 destruct (make_rmap _ H1 (level phi1)) as [phi' [? ?]].
 clear H1.
@@ -1017,7 +950,6 @@ inv H1.
 simpl; f_equal.
 pose proof (resource_at_approx phi1 loc). rewrite H0 in H1. simpl in H1.
 injection H1; intros; auto.
-inv H1; auto.
 (*  End of make_rmap proof *)
 exists phi'.
 apply resource_at_join2; auto.
@@ -1040,7 +972,7 @@ Proof.
 Qed.
 
 Definition no_preds (r: resource) :=
-   match r with NO _ _ => True | YES _ _ _ pp => pp=NoneP | PURE _ pp => pp=NoneP | GHOST _ => True end.
+   match r with NO _ _ => True | YES _ _ _ pp => pp=NoneP | PURE _ pp => pp=NoneP end.
 
 Lemma remake_rmap:
   forall (f: AV.address -> resource),
@@ -1320,7 +1252,7 @@ Definition res_retain (r: resource) : Share.t :=
  match r with
   | NO sh _ => retainer_part sh
   | YES sh _ _ _ => retainer_part sh
-  | PURE _ _ | GHOST _ => Share.bot
+  | PURE _ _ => Share.bot
  end.
 
 Lemma fixup_trace_readable:
@@ -1350,8 +1282,7 @@ Qed.
             | Some(sh,k), PURE _ pp =>
                YES _ (fixup_trace_readable (retain x) sh) k pp
             | Some (sh,k), YES _ _ _ pp => YES _ (fixup_trace_readable (retain x) sh) k pp
-            | Some (sh, k), NO _ _ | Some (sh, k), GHOST _ => YES _ (fixup_trace_readable (retain x) sh) k NoneP
-            | None, GHOST _ => gtrace x
+            | Some (sh, k), NO _ _ => YES _ (fixup_trace_readable (retain x) sh) k NoneP
             | None, _ => NO _ (@retainer_part_nonreadable (retain x))
             end.
 
@@ -1728,7 +1659,7 @@ Proof.
 Qed.*)
 
 Lemma identity_resource: forall r: resource, identity r <->
-    match r with YES _ _ _ _ => False | NO sh rsh => identity sh | PURE _ _ => True | GHOST m => identity m end.
+    match r with YES _ _ _ _ => False | NO sh rsh => identity sh | PURE _ _ => True end.
 Proof.
  intros. destruct r.
  - split; intro.
@@ -1743,10 +1674,6 @@ Proof.
    specialize (H (NO Share.bot bot_unreadable) (YES sh r k p)).
    spec H. constructor. apply join_unit2; auto. inv H.
  - intuition. intros  ? ? ?. inv H0. auto.
- - split; [|apply GHOST_identity].
-   intro; apply empty_NO in H.
-   destruct H as [? | [[? []] | [? []]]]; try discriminate.
-   inv H; auto.
 Qed.
 
 Lemma resource_at_core_identity:  forall m i, identity (core m @ i).
@@ -1760,8 +1687,6 @@ Proof.
   clear - r RJ.
   apply unit_identity in RJ. apply identity_share_bot in RJ.
   subst. apply bot_unreadable in r. auto.
-  rewrite H in Hdup; inv Hdup.
-  apply identity_unit_equiv; auto.
 Qed.
 
 Lemma YES_inj: forall sh rsh k pp sh' rsh' k' pp',
@@ -1800,10 +1725,9 @@ Lemma resource_at_identity: forall (m: rmap) (loc: AV.address),
  identity m -> identity (m @ loc).
 Proof.
   intros.
-  destruct (@resource_at_empty m H loc) as [?|[[? [? ?]] | [? []]]].
+  destruct (@resource_at_empty m H loc) as [?|[? [? ?]]].
   rewrite H0. apply NO_identity.
   rewrite H0. apply PURE_identity.
-  rewrite H0. apply GHOST_identity; auto.
 Qed.
 
 Lemma core_YES: forall sh rsh k pp, core (YES sh rsh k pp) = NO Share.bot bot_unreadable.
@@ -1836,14 +1760,6 @@ Proof.
  inv H; auto.
 Qed.
 
-Lemma core_GHOST: forall m, core (GHOST m) = GHOST (core m).
-Proof.
- intros. pose proof (core_unit (GHOST m)) as H; inv H.
- apply f_equal.
- erewrite <- join_core by eauto.
- eapply identity_core, unit_identity; eauto.
-Qed.
-
 Lemma core_not_YES: forall {w loc rsh sh k pp},
    core w @ loc = YES rsh sh k pp -> False.
 Proof.
@@ -1870,7 +1786,7 @@ Lemma resource_fmap_core:
 Proof.
 intros.
 case_eq (w @ loc); intros;
- [rewrite core_NO | rewrite core_YES | rewrite core_PURE | rewrite core_GHOST]; auto.
+ [rewrite core_NO | rewrite core_YES | rewrite core_PURE]; auto.
 rewrite <- H. apply resource_at_approx.
 Qed.
 
