veric/slice.v
@@ -75,7 +75,6 @@ Definition split_resource r :=
                (YES (fst (Share.split sh)) (split_YES_ok1 _ rsh) k pp , 
                 YES (snd (Share.split sh)) (split_YES_ok2 _ rsh) k pp)
              | PURE k pp => (PURE k pp, PURE k pp)
-             | GHOST m => (GHOST (core m), GHOST m)
              | NO sh nsh => (NO (fst (Share.split sh)) (split_NO_ok1 _ nsh),
                              NO (snd (Share.split sh)) (split_NO_ok2 _ nsh))
   end.
@@ -177,7 +176,6 @@ Lemma split_resource_join: forall r, join (fst (split_resource r)) (snd (split_r
 Proof.
 intro.
 destruct r; simpl; constructor; auto; try (apply split_join; apply surjective_pairing).
-apply core_unit.
 Qed.
 
 Lemma split_rmap_join:
@@ -225,7 +223,6 @@ Definition slice_resource (sh: share) (r: resource) : resource :=
     | right n => NO sh n
     end
    | PURE k pp => PURE k pp
-   | GHOST m => GHOST m
   end.
 
 Lemma slice_resource_valid:
@@ -327,7 +324,6 @@ rewrite H7.
 f_equal. apply proof_irr.
 apply join_level in H1; intuition.
 congruence.
-congruence.
 (* noat case *)
 generalize (resource_at_join _ _ _ l' H1); intro.
 apply split_identity in H3; auto.
@@ -341,7 +337,7 @@ Proof.
  assert (sh = retainer_part Share.bot).
    unfold retainer_part. rewrite Share.glb_bot.
    apply identity_NO in H.
-   destruct H as [|[|]]. inv H. auto. destruct H as [? [? ?]]. inv H. destruct H as [? []]. inv H.
+   destruct H as [|]. inv H. auto. destruct H as [? [? ?]]. inv H.
    subst; f_equal. apply proof_irr.
    apply YES_not_identity in H. contradiction.
 Qed.
@@ -592,7 +588,6 @@ Definition share_oblivious (P: pred rmap) :=
                  | NO _ _, NO _ _ => True
                  | YES _ sh1 k1 p1 , YES _ sh2 k2 p2 => k1=k2 /\ p1=p2
                  | PURE k1 p1, PURE k2 p2 => k1=k2 /\ p1=p2
-                 | GHOST _, GHOST _ => True
                  | _ , _ => False
                  end) ->
      P w' -> P w.
@@ -632,7 +627,6 @@ inversion2 H9 H13.
 do 3 red in H4. rewrite H11 in H4.
 contradiction (YES_not_identity _ _ _ _ H4).
 rewrite H11 in H10; inv H10.
-rewrite H11 in H10; inv H10.
 destruct (w1 @ l0); inv H10; auto.
 inv H10; auto.
 destruct H3 as [[w1 [w2 [? [? ?]]]] ?].
@@ -657,7 +651,6 @@ destruct H5 as [? [? [? ?]]].
 congruence.
 do 3 red in H5. rewrite H10 in H5. 
 contradiction (YES_not_identity _ _ _ _ H5).
-rewrite H10 in H9; inv H9.
 rewrite H10 in H9; inv H9.
 inv H9; auto.
 inv H9; auto.
@@ -759,8 +752,6 @@ Proof.
   contradiction (join_unreadable_shares H n n0).
 *
   constructor.
-*
-  discriminate.
 Qed.
 
 Definition resource_share_split (p q r: address -> pred rmap): Prop :=
@@ -1137,7 +1128,6 @@ Proof.
       apply YES_ext.
       eapply join_eq; eauto.
     - inv H1. inv H0. apply YES_ext. eapply join_eq; eauto.
-    - inv H1.
     - inv H1.
 Qed.
 
